pulse/lib/pulse_core/PulseCore.InstantiatedSemantics.fst
@@ -1,0 +1,77 @@
+module PulseCore.InstantiatedSemantics
+module Sem = PulseCore.Semantics2
+module Mem = PulseCore.Memory
+
+let laws ()
+: squash (
+    Sem.associative Mem.star /\
+    Sem.commutative Mem.star /\
+    Sem.is_unit Mem.emp Mem.star
+  )
+= let open Mem in
+  let equiv_eq (x y:slprop)
+    : Lemma (x `equiv` y <==> x == y)
+          [SMTPat (x `equiv` y)]
+    = introduce x `equiv` y ==> x == y
+      with _h . Mem.slprop_extensionality x y
+  in
+  let _ : squash (Sem.associative star) =
+    introduce 
+        forall x y z. 
+            ((x `star` y) `star` z) ==
+            (x `star` (y `star` z))
+    with Mem.star_associative x y z
+  in
+  let _ : squash (Sem.commutative star) = 
+    introduce 
+        forall x y.
+            x `star` y == y `star` x
+        with Mem.star_commutative x y
+  in
+  let _ : squash (Sem.is_unit emp star) =
+    introduce
+        forall x.
+            (x `star` emp) == x /\
+            (emp `star` x) == x
+        with Mem.emp_unit x
+  in
+  ()
+
+let state : Sem.state = {
+    s = Mem.mem;
+    is_full_mem = Mem.full_mem_pred;
+    pred = Mem.slprop;
+    emp = Mem.emp;
+    star = Mem.star;
+    interp = Mem.interp;
+    evolves = Mem.mem_evolves;
+    invariant = Mem.locks_invariant Set.empty;
+    laws = laws ()
+}
+
+let stt (a:Type u#a) 
+        (pre:Mem.slprop)
+        (post:a -> Mem.slprop)
+: Type0
+= unit -> Dv (Sem.m u#2 u#a #state a pre post)
+
+let return (#a:Type u#a) (x:a) (p:a -> Mem.slprop)
+: stt a (p x) p
+= fun _ -> Sem.ret x p
+
+open Mem
+let bind_stt
+    (#a:Type u#a) (#b:Type u#b)
+    (#pre1:slprop) (#post1:a -> slprop) (#post2:b -> slprop)
+    (e1:stt a pre1 post1)
+    (e2:(x:a -> stt b (post1 x) post2))
+: stt b pre1 post2
+= fun _ -> Sem.mbind (e1()) (fun x -> e2 x ())
+
+let frame_stt
+  (#a:Type u#a)
+  (#pre:slprop) (#post:a -> slprop)
+  (frame:slprop)
+  (e:stt a pre post)
+: stt a (pre `star` frame) (fun x -> post x `star` frame)
+= fun _ -> Sem.frame frame (e())
